Added some comments

Congruence_Closure.thy
@@ -4,40 +4,63 @@ theory Congruence_Closure
     Explain_Proofs2 
 begin
 
-datatype 'a equation = Constants 'a 'a ("_ \<approx> _")
-  | Function 'a 'a 'a                 ("F _ _ \<approx> _" )
+section \<open>Definitions\<close>
 
-datatype 'a pending_equation = One "'a equation"
-  | Two "'a equation" "'a equation"
+text \<open>The input equations to this congruence closure algorithm need 
+      to be curryfied and flattened into terms of depth at most 2,
+      by introducing the "apply" function \<open>f\<close> and new constants.
+      
+      The constants of the equation are represented by natural numbers,
+      so that they can be also used as index of the union-find array.
+      Each natural number represents an arbitrary constant, 
+      which is not related to the number it is represented by.
+
+      For example the equation \<open>2 \<approx> 5\<close> should be interpreted as \<open>c\<^sub>2 = c\<^sub>5\<close>.\<close>
+datatype equation = Constants nat nat ("_ \<approx> _")
+  | Function nat nat nat                 ("F _ _ \<approx> _" )
+
+datatype pending_equation = One equation
+  | Two equation equation
 
 term "a \<approx> b"
 term "F a b \<approx> c"
 
+text \<open>Data structure for the congruence closure operations (merge, are_congruent and explain):
+  \<open>cc_list\<close>: parents of the union-find-like tree data structure without path compression
+  \<open>class_list\<close>: stores for each representative a list with all the constants of the class (maybe not useful) 
+  \<open>use_list\<close>: for each representative \<open>a\<close>, a list if input equations \<open>f b\<^sub>1 b\<^sub>2 = b\<close>,
+              where \<open>a\<close> is the representative of either \<open>b\<^sub>1\<close> or \<open>b\<^sub>2\<close>.
+  \<open>lookup\<close>: table indexed by pairs of representatives \<open>b\<close> and \<open>c\<close>, 
+            which stores an input equation \<open>f a\<^sub>1 a\<^sub>2 = a\<close> s.t.
+            \<open>b\<close> and \<open>c\<close> are representatives of \<open>a\<^sub>1\<close> and \<open>a\<^sub>2\<close> respectively,
+            or None if no such equation exists.
+  \<open>proof_forest\<close>: tree-shaped graph, with the sequence of merge operations as edges
+  \<open>pf_labels\<close>: for each edge in the \<open>proof_forest\<close>, a label with the input equations
+\<close>
 record congruence_closure =
-  uf_list :: "nat list"
+  cc_list :: "nat list"
   class_list :: "nat list list"
-  use_list :: "nat equation list list"
-  lookup :: "nat equation option list list"
+  use_list :: "equation list list"
+  lookup :: "equation option list list"
 
-
-fun lookup_Some :: "nat equation option list list \<Rightarrow> nat equation \<Rightarrow> bool"
+fun lookup_Some :: "equation option list list \<Rightarrow> equation \<Rightarrow> bool"
   where
 "lookup_Some t (F a\<^sub>1 a\<^sub>2 \<approx> a) = (\<not>Option.is_none ((t ! a\<^sub>1) ! a\<^sub>2))"
 | "lookup_Some t (a \<approx> b) = False"
 
-fun lookup_None :: "nat equation option list list \<Rightarrow> nat equation \<Rightarrow> bool"
+fun lookup_None :: "equation option list list \<Rightarrow> equation \<Rightarrow> bool"
   where
 "lookup_None t (F a\<^sub>1 a\<^sub>2 \<approx> a) = (Option.is_none ((t ! a\<^sub>1) ! a\<^sub>2))"
 | "lookup_None t (a \<approx> b) = False"
 
 \<comment> \<open>Should only be used if \<open>lookup(a\<^sub>1, a\<^sub>2)\<close> is not None and if the equation is not of the type (a = b)\<close>
-fun link_to_lookup :: "nat equation option list list \<Rightarrow> nat equation \<Rightarrow> nat pending_equation"
+fun link_to_lookup :: "equation option list list \<Rightarrow> equation \<Rightarrow> pending_equation"
   where
 "link_to_lookup t (F a\<^sub>1 a\<^sub>2 \<approx> a) = Two (F a\<^sub>1 a\<^sub>2 \<approx> a) (the ((t ! a\<^sub>1) ! a\<^sub>2))"
   \<comment> \<open>This should not be invoked.\<close>
 | "link_to_lookup t (a \<approx> b) = One (a \<approx> b)"
 
-function set_lookup :: "nat equation option list list \<Rightarrow> nat equation list \<Rightarrow> nat list \<Rightarrow> nat equation option list list"
+function set_lookup :: "equation option list list \<Rightarrow> equation list \<Rightarrow> nat list \<Rightarrow> equation option list list"
   where
 "set_lookup t [] l = t"
 | "set_lookup t ((F a\<^sub>1 a\<^sub>2 \<approx> a)#xs) l = 
@@ -49,14 +72,14 @@ function set_lookup :: "nat equation option list list \<Rightarrow> nat equation
 termination by lexicographic_order
 
 function propagate_one :: "congruence_closure \<Rightarrow> nat \<Rightarrow> nat \<Rightarrow> congruence_closure"
-and propagate :: "nat pending_equation list \<Rightarrow> congruence_closure \<Rightarrow> congruence_closure"
+and propagate :: "pending_equation list \<Rightarrow> congruence_closure \<Rightarrow> congruence_closure"
   where
-"propagate_one \<lparr>uf_list = l, class_list = c, use_list = u, lookup = t\<rparr> a b =  
+"propagate_one \<lparr>cc_list = l, class_list = c, use_list = u, lookup = t\<rparr> a b =  
 (if rep_of l a = rep_of l b 
-    then \<lparr>uf_list = l, class_list = c, use_list = u, lookup = t\<rparr>
+    then \<lparr>cc_list = l, class_list = c, use_list = u, lookup = t\<rparr>
   else 
     propagate (map (link_to_lookup t) (filter (lookup_Some t) (u ! rep_of l a)))
-    \<lparr>uf_list = ufa_union l a b, 
+    \<lparr>cc_list = ufa_union l a b, 
     class_list = (c[rep_of l a := []])[rep_of l b := (c ! rep_of l b) @ (c ! rep_of l a)],
     use_list = (u[rep_of l a := []])[rep_of l b := (u ! rep_of l b) @ (filter (lookup_None t) (u ! rep_of l a))], 
     lookup = set_lookup t (filter (lookup_None t) (u ! rep_of l a)) l\<rparr>
@@ -77,30 +100,42 @@ and propagate :: "nat pending_equation list \<Rightarrow> congruence_closure \<R
   by pat_completeness auto
 
 
-function merge:: "congruence_closure \<Rightarrow> nat equation \<Rightarrow> congruence_closure"
+function merge:: "congruence_closure \<Rightarrow> equation \<Rightarrow> congruence_closure"
   where 
-"merge \<lparr>uf_list = l, class_list = c, use_list = u, lookup = t\<rparr> (a \<approx> b) = 
-propagate [One (a \<approx> b)] \<lparr>uf_list = l, class_list = c, use_list = u, lookup = t\<rparr>"
+"merge \<lparr>cc_list = l, class_list = c, use_list = u, lookup = t\<rparr> (a \<approx> b) = 
+propagate [One (a \<approx> b)] \<lparr>cc_list = l, class_list = c, use_list = u, lookup = t\<rparr>"
 
-| "merge \<lparr>uf_list = l, class_list = c, use_list = u, lookup = t\<rparr> (F a\<^sub>1 a\<^sub>2 \<approx> a) = 
+| "merge \<lparr>cc_list = l, class_list = c, use_list = u, lookup = t\<rparr> (F a\<^sub>1 a\<^sub>2 \<approx> a) = 
 (case (t ! rep_of l a\<^sub>1) ! rep_of l a\<^sub>2 of
 Some eq 
-      \<Rightarrow> propagate [Two (F a\<^sub>1 a\<^sub>2 \<approx> a) eq] \<lparr>uf_list = l, class_list = c, use_list = u, lookup = t\<rparr>
+      \<Rightarrow> propagate [Two (F a\<^sub>1 a\<^sub>2 \<approx> a) eq] \<lparr>cc_list = l, class_list = c, use_list = u, lookup = t\<rparr>
 | None 
-      \<Rightarrow> \<lparr>uf_list = l, class_list = c, 
+      \<Rightarrow> \<lparr>cc_list = l, class_list = c, 
 use_list = (u[rep_of l a\<^sub>1 := (F a\<^sub>1 a\<^sub>2 \<approx> a)#(u ! rep_of l a\<^sub>1)])[rep_of l a\<^sub>2 := (F a\<^sub>1 a\<^sub>2 \<approx> a)#(u ! rep_of l a\<^sub>2)], 
 lookup = t[rep_of l a\<^sub>1 := (t ! rep_of l a\<^sub>1)[rep_of l a\<^sub>2 := Some (F a\<^sub>1 a\<^sub>2 \<approx> a)]]\<rparr>
 )"
   by pat_completeness auto
 
-fun are_congruent :: "congruence_closure \<Rightarrow> nat equation \<Rightarrow> bool"
+fun are_congruent :: "congruence_closure \<Rightarrow> equation \<Rightarrow> bool"
   where
-"are_congruent \<lparr>uf_list = l, class_list = c, use_list = u, lookup = t\<rparr> (a \<approx> b) = 
+"are_congruent \<lparr>cc_list = l, class_list = c, use_list = u, lookup = t\<rparr> (a \<approx> b) = 
     (rep_of l a = rep_of l b)"
-| "are_congruent \<lparr>uf_list = l, class_list = c, use_list = u, lookup = t\<rparr> (F a\<^sub>1 a\<^sub>2 \<approx> a) = 
+| "are_congruent \<lparr>cc_list = l, class_list = c, use_list = u, lookup = t\<rparr> (F a\<^sub>1 a\<^sub>2 \<approx> a) = 
     (case (t ! rep_of l a\<^sub>1) ! rep_of l a\<^sub>2 of
       Some (F b\<^sub>1 b\<^sub>2 \<approx> b) \<Rightarrow> (rep_of l a = rep_of l b)
     | None \<Rightarrow> False
 )"
+
+text \<open>Implementation of the proof forest\<close>
+
+function add_edge :: "nat list \<Rightarrow> nat \<Rightarrow> nat \<Rightarrow> nat list"
+  where
+"add_edge pf e e' = (if pf ! e = e then (pf[e := e']) else add_edge (pf[e := e']) (pf ! e) e)"
+  by pat_completeness auto
+
+text \<open>For the initialisation of the congruence closure algorithm.\<close>
+abbreviation 
+"initial_cc n \<equiv> \<lparr>cc_list = [0..<n], class_list = replicate n [], use_list = replicate n [], lookup = replicate n (replicate n None)\<rparr>"
+
 
 end
